NBE/SingleSortImp/BetaEta.lean
@@ -1,0 +1,1567 @@
+import NBE.Rel
+import NBE.Map
+import NBE.SingleSortImp.Beta
+
+namespace SingleSortImp
+
+/-!
+### equalities between Morphisms
+-/
+
+
+inductive Tm.step: Tm -> Tm -> Prop where
+  -- beta reduction
+  | appAbs {t s: Tm}: Tm.step (.app t.abs s) (t.subst 0 s.up0).down0
+  -- eta reduction
+  | eta {t: Tm}: Tm.step (t.up0.app $ .var 0).abs t
+  -- congrunence relation
+  | abs {t1 t2: Tm}: Tm.step t1 t2 -> Tm.step t1.abs t2.abs
+  | app1 {t1 t2 s: Tm}: Tm.step t1 t2 -> Tm.step (.app t1 s) (.app t2 s)
+  | app2 {t s1 s2: Tm}: Tm.step s1 s2 -> Tm.step (.app t s1) (.app t s2)
+
+
+def Tm.mstep: Tm -> Tm -> Prop := RTCl Tm.step
+def Tm.eq := ECl Tm.step
+def Tm.normal := Relation.Normal Tm.step
+
+
+
+theorem Tm.mstep.abs {t1 t2: Tm}:
+  t1.mstep t2 -> t1.abs.mstep t2.abs
+:= by
+  apply RTCl.keep_cong Tm.step.abs
+
+
+theorem Tm.mstep.app1 {t1 t2 s: Tm}:
+  t1.mstep t2 -> (t1.app s).mstep (t2.app s)
+:= by
+  apply RTCl.keep_cong Tm.step.app1
+
+
+theorem Tm.mstep.app2 {t s1 s2: Tm}:
+  s1.mstep s2 -> (t.app s1).mstep (t.app s2)
+:= by
+  apply RTCl.keep_cong Tm.step.app2
+
+
+theorem Tm.mstep.app {t1 t2 s1 s2: Tm}:
+  t1.mstep t2 ->
+  s1.mstep s2 ->
+  (t1.app s1).mstep (t2.app s2)
+:= by
+  intro St Ss
+  apply RTCl.trans
+  . apply Tm.mstep.app1
+    exact St
+  . apply Tm.mstep.app2
+    exact Ss
+
+
+theorem Tm.eq.abs {t1 t2: Tm}:
+  t1.eq t2 -> t1.abs.eq t2.abs
+:= by
+  apply ECl.keep_cong Tm.step.abs
+
+
+theorem Tm.eq.app1 {t1 t2 s: Tm}:
+  t1.eq t2 -> (t1.app s).eq (t2.app s)
+:= by
+  apply ECl.keep_cong Tm.step.app1
+
+
+theorem Tm.eq.app2 {t s1 s2: Tm}:
+  s1.eq s2 -> (t.app s1).eq (t.app s2)
+:= by
+  apply ECl.keep_cong Tm.step.app2
+
+
+theorem Tm.eq.app {t1 t2 s1 s2: Tm}:
+  t1.eq t2 -> s1.eq s2 -> (t1.app s1).eq (t2.app s2)
+:= by
+  intro H1 H2
+  apply ECl.trans
+  . apply H1.app1
+  . apply H2.app2
+
+
+theorem Tm.step.typing {Γ: Context} {t t': Tm} {T}:
+  t.step t' -> Γ.Typing t T -> Γ.Typing t' T
+:= by
+  intro S HT
+  induction HT generalizing t' with
+  | var H =>
+    cases S
+  | abs H IH =>
+    cases S with
+    | abs S =>
+      specialize IH S
+      constructor
+      exact IH
+    | eta =>
+      cases H with | app H1 H2 =>
+      cases H2 with | var H2 =>
+      simp_all
+      apply Context.weaken_cons_inv
+      apply H1
+  | app H1 H2 IH1 IH2 =>
+    cases S with
+    | appAbs =>
+      cases H1
+      apply Context.subst_typing
+      . assumption
+      . exact H2
+    | app1 S =>
+      constructor
+      . apply IH1
+        exact S
+      . exact H2
+    | app2 S =>
+      constructor
+      . exact H1
+      . apply IH2
+        exact S
+
+
+theorem Tm.mstep.typing {Γ: Context} {t t': Tm} {T}:
+  t.mstep t' -> Γ.Typing t T -> Γ.Typing t' T
+:= by
+  intro S HT
+  induction S with
+  | refl =>
+    apply HT
+  | step Hxy Hyz IH =>
+    apply IH
+    apply Hxy.typing
+    exact HT
+
+
+mutual
+  inductive Tm.NE: Context -> Tm -> Ty -> Prop where
+    | var {Γ: Context} {x} {T}: Γ.lookup x = some T -> Tm.NE Γ (.var x) T
+    | app {Γ} {t s} {T1 T2}: Tm.NE Γ t (T1.imp T2) -> Tm.NF Γ s T1 -> Tm.NE Γ (t.app s) T2
+
+  inductive Tm.NF: Context -> Tm -> Ty -> Prop where
+    | atom {Γ} {t}: Tm.NE Γ t .Atom -> Tm.NF Γ t .Atom
+    | abs {Γ} {t} {T1 T2}: Tm.NF (T1 :: Γ) t T2 -> Tm.NF Γ t.abs (T1.imp T2)
+end
+
+
+theorem Tm.NFNE.typing {Γ: Context} {t T}:
+  (Tm.NF Γ t T -> Γ.Typing t T) ∧ (Tm.NE Γ t T -> Γ.Typing t T)
+:= by
+  induction t generalizing Γ T with
+  | _ =>
+    grind [Tm.NF, Tm.NE, Context.Typing]
+
+
+theorem Tm.NF.typing {Γ: Context} {t T}:
+  Tm.NF Γ t T -> Γ.Typing t T
+:= by
+  apply Tm.NFNE.typing.left
+
+theorem Tm.NE.typing {Γ: Context} {t T}:
+  Tm.NE Γ t T -> Γ.Typing t T
+:= by
+  apply Tm.NFNE.typing.right
+
+
+theorem Tm.N_weakening {Γ2 Γ3 Γ1 T} {t: Tm}:
+  (Tm.NE (Γ2 ++ Γ1) t T <-> Tm.NE (Γ2 ++ (Γ3 ++ Γ1)) (t.up Γ2.length Γ3.length) T) ∧
+  (Tm.NF (Γ2 ++ Γ1) t T <-> Tm.NF (Γ2 ++ (Γ3 ++ Γ1)) (t.up Γ2.length Γ3.length) T)
+:= by
+  induction t generalizing Γ1 Γ2 Γ3 T with
+  | var x =>
+    and_intros
+    . apply Iff.intro
+      . intro N
+        cases N with | var H =>
+        constructor
+        split
+        . grind [FinMap.lookup]
+        . have I: x ≥ Γ2.length := by omega
+          simp [FinMap.lookup_right I] at H
+          have I: x + Γ3.length ≥ Γ2.length := by omega
+          simp [FinMap.lookup_right I]
+          grind [FinMap.lookup]
+      . intro N
+        cases N with | var H =>
+        constructor
+        split at H
+        . grind [FinMap.lookup]
+        . have I: x ≥ Γ2.length := by omega
+          simp [FinMap.lookup_right I]
+          have I: x + Γ3.length ≥ Γ2.length := by omega
+          simp [FinMap.lookup_right I] at H
+          grind [FinMap.lookup]
+    . apply Iff.intro
+      . intro N
+        cases N with | atom N =>
+        cases N with | var H =>
+        constructor
+        constructor
+        split
+        . grind [FinMap.lookup]
+        . next I =>
+          have I: x ≥ Γ2.length := by omega
+          simp [FinMap.lookup_right I] at H
+          have I: x + Γ3.length ≥ Γ2.length := by omega
+          simp [FinMap.lookup_right I]
+          grind [FinMap.lookup]
+      . intro N
+        cases N with | atom N =>
+        cases N with | var H =>
+        constructor
+        constructor
+        split at H
+        . grind [FinMap.lookup]
+        . have I: x ≥ Γ2.length := by omega
+          simp [FinMap.lookup_right I]
+          have I: x + Γ3.length ≥ Γ2.length := by omega
+          simp [FinMap.lookup_right I] at H
+          grind [FinMap.lookup]
+  | app t1 t2 IH1 IH2 =>
+    and_intros
+    . apply Iff.intro
+      . intro N
+        cases N with | app N1 N2 =>
+        constructor
+        . apply IH1.left.mp
+          exact N1
+        . apply IH2.right.mp
+          exact N2
+      . intro N
+        cases N with | app N1 N2 =>
+        constructor
+        . apply IH1.left.mpr
+          exact N1
+        . apply IH2.right.mpr
+          exact N2
+    . apply Iff.intro
+      . intro N
+        cases N with | atom N =>
+        cases N with | app N1 N2 =>
+        constructor
+        constructor
+        . apply IH1.left.mp
+          exact N1
+        . apply IH2.right.mp
+          exact N2
+      . intro N
+        cases N with | atom N =>
+        cases N with | app N1 N2 =>
+        constructor
+        constructor
+        . apply IH1.left.mpr
+          exact N1
+        . apply IH2.right.mpr
+          exact N2
+  | abs M IH =>
+    and_intros
+    . apply Iff.intro
+      . intro N
+        cases N
+      . intro N
+        cases N
+    . apply Iff.intro
+      . intro N
+        cases N with
+        | atom N => cases N
+        | abs N =>
+          constructor
+          grind [Tm.NE, Tm.NF]
+      . intro N
+        cases N with
+        | atom N => cases N
+        | abs N =>
+          constructor
+          grind [Tm.NE, Tm.NF]
+
+
+theorem Tm.NE.weaken_app {Γ' Γ T} {t: Tm}:
+  Tm.NE Γ t T -> Tm.NE (Γ' ++ Γ) (t.up 0 Γ'.length) T
+:= by
+  let H := (Tm.N_weakening (Γ2 := []) (Γ3 := Γ') (Γ1 := Γ) (t := t) (T := T))
+  simp at H
+  apply H.left.mp
+
+
+theorem Tm.NF.weaken_app {Γ' Γ T} {t: Tm}:
+  Tm.NF Γ t T -> Tm.NF (Γ' ++ Γ) (t.up 0 Γ'.length) T
+:= by
+  let H := (Tm.N_weakening (Γ2 := []) (Γ3 := Γ') (Γ1 := Γ) (t := t) (T := T))
+  simp at H
+  apply H.right.mp
+
+
+/-!
+We know some facts about reduction. We first need the following lemma to perform a
+`step` operation.
+-/
+
+/--
+This is trivial, but there could be some situation that the `t` is not `step` to a
+substitution. Then, you can apply this theorem to intro the `t'` in order to do the computation.
+-/
+theorem Tm.step.compute {t t' t'': Tm}:
+  t.step t' -> t' = t'' -> t.step t''
+:= by
+  intro H E
+  simp_all
+
+
+theorem Tm.step.appAbs_ssubst {t s: Tm}:
+  (t.abs.app s).step (t.ssubst (.step s))
+:= by
+  apply Tm.step.compute
+  . apply Tm.step.appAbs
+  . apply Tm.step_ssubst
+
+
+@[simp]
+theorem Tm.up0_ssubst_abs {t: Tm} {s: Subst}:
+  (t.up0.ssubst s.abs) = (t.ssubst s).up0
+:= by
+  unfold up0
+  simp [Tm.up_ssubst]
+  apply Tm.ssubst_congr
+  intro n
+  simp [Subst.comp]
+  cases n with
+  | _ =>
+    simp [Tm.ssubst, Subst.up, Subst.abs]
+    unfold up0
+    simp [Tm.up_ssubst]
+
+
+theorem Tm.step.ssubst {t1 t2: Tm} {s: Subst}:
+  t1.step t2 ->
+  (t1.ssubst s).step (t2.ssubst s)
+:= by
+  intro S
+  induction S generalizing s with
+  | appAbs =>
+    rename_i t11 t12
+    rewrite [Tm.step_ssubst]
+    simp [Tm.ssubst]
+    apply Tm.step.compute
+    . apply Tm.step.appAbs_ssubst
+    simp
+    apply Tm.ssubst_congr
+    intro n
+    simp [Subst.comp]
+    cases n with
+    | zero =>
+      simp [Subst.step, Subst.abs, Tm.ssubst]
+    | succ m =>
+      simp [Subst.step, Subst.abs, Tm.ssubst]
+  | eta =>
+    simp [Tm.ssubst, Subst.abs]
+    rename_i t
+    apply eta
+  | abs S IH =>
+    constructor
+    apply IH
+  | app1 S IH =>
+    apply Tm.step.app1
+    apply IH
+  | app2 S IH =>
+    apply Tm.step.app2
+    apply IH
+
+
+
+/--
+The shift is congruent over `step`
+-/
+theorem Tm.step.up {c n} {t t': Tm}:
+  t.step t' -> (t.up c n).step (t'.up c n)
+:= by
+  simp [Tm.up_ssubst]
+  apply Tm.step.ssubst
+
+
+theorem Tm.mstep.up {c n} {t t': Tm}:
+  t.eq t' -> (t.up c n).eq (t'.up c n)
+:= by
+  intro S
+  apply ECl.keep_cong Tm.step.up
+  exact S
+
+
+theorem Tm.eq.up {c n} {t t': Tm}:
+  t.eq t' -> (t.up c n).eq (t'.up c n)
+:= by
+  intro S
+  apply ECl.keep_cong Tm.step.up
+  exact S
+
+
+theorem Tm.step.down {c} {t t': Tm}:
+  t.step t' -> (t.down c).step (t'.down c)
+:= by
+  simp [Tm.down_ssubst]
+  apply Tm.step.ssubst
+
+
+theorem Tm.mstep.down {c} {t t': Tm}:
+  t.mstep t' -> (t.down c).mstep (t'.down c)
+:= by
+  apply RTCl.keep_cong Tm.step.down
+
+
+theorem Tm.eq.down {c} {t t': Tm}:
+  t.eq t' -> (t.down c).eq (t'.down c)
+:= by
+  apply ECl.keep_cong Tm.step.down
+
+
+theorem Tm.mstep.up_down {t t': Tm}:
+  t.up0.mstep t' -> t.mstep t'.down0
+:= by
+  intro H
+  replace H := Tm.mstep.down H (c := 0)
+  simp [Tm.up0] at H
+  exact H
+
+
+theorem Tm.BNE.BNF {t: Tm}:
+  t.BNE -> t.BNF
+:= by
+  intro H
+  constructor
+  exact H
+
+
+theorem Tm.BN.up {t: Tm} {c n}:
+  (t.BNE <-> (t.up c n).BNE) ∧ (t.BNF <-> (t.up c n).BNF)
+:= by
+  induction t generalizing c n <;>
+  grind [up, BNE, BNF]
+
+
+theorem Tm.step.BN {t s: Tm}:
+  t.step s ->
+  (t.BNE -> s.BNE) ∧ (t.BNF -> s.BNF)
+:= by
+  intro S
+  induction S with try grind [BNE, BNF]
+  | eta =>
+    rename_i t
+    and_intros
+    . intro N
+      cases N
+    . intro N
+      cases N <;> try contradiction
+      rename_i N
+      cases N <;> try contradiction
+      rename_i N
+      cases N with | app N _ =>
+      apply BNF.neutral
+      apply BN.up.left.mpr
+      exact N
+
+
+theorem Tm.step.BNE {t s: Tm}:
+  t.step s ->
+  (t.BNE -> s.BNE)
+:= by
+  intro S
+  apply S.BN.left
+
+
+theorem Tm.step.BNF {t s: Tm}:
+  t.step s ->
+  (t.BNF -> s.BNF)
+:= by
+  intro S
+  apply S.BN.right
+
+
+theorem Tm.mstep.BNE {t s: Tm}:
+  t.mstep s ->
+  t.BNE ->
+  s.BNE
+:= by
+  intro S N
+  induction S with
+  | refl =>
+    exact N
+  | step Hty Hys IH =>
+    apply IH
+    apply Hty.BN.left
+    exact N
+
+
+def Tm.freeVar (x: Nat): Tm -> Bool
+  | .var y => y = x
+  | .app t1 t2 => t1.freeVar x || t2.freeVar x
+  | .abs t => t.freeVar (x + 1)
+
+
+theorem Tm.not_free_up {t: Tm} {c n: Nat}:
+  (forall i: Nat, c ≤ i -> i < c + n -> t.freeVar i = false) ->
+  exists s: Tm, t = s.up c n
+:= by
+  intro H
+  induction t generalizing c n with
+  | var x =>
+    simp [freeVar] at H
+    obtain E1 | E2 : x < c ∨ x ≥ c := by omega
+    . exists (.var x)
+      simp [up]
+      grind
+    . exists .var (x - n)
+      simp [up]
+      grind
+  | app t1 t2 IH1 IH2 =>
+    simp [freeVar] at H
+    obtain ⟨s1, E1⟩ := IH1 (fun i h1 h2 => (H i h1 h2).left)
+    obtain ⟨s2, E2⟩ := IH2 (fun i h1 h2 => (H i h1 h2).right)
+    exists s1.app s2
+    simp_all [up]
+  | abs t IH =>
+    simp [freeVar] at H
+    replace H: forall i: Nat, c + 1 ≤ i -> i < (c + 1) + n -> t.freeVar i = false := by
+      intro i H1 H2
+      have E: i = (i - 1) + 1 := by omega
+      rewrite [E]
+      grind
+    obtain ⟨s, E⟩ := IH H
+    exists s.abs
+    simp_all [up]
+
+
+theorem Tm.not_free_up0 {t: Tm}:
+  t.freeVar 0 = false ->
+  exists s: Tm, t = s.up0
+:= by
+  intro H
+  apply Tm.not_free_up
+  simp_all
+
+
+theorem Tm.free_not_up {c n} {t s: Tm}:
+  (exists i: Nat, c ≤ i ∧ i < c + n ∧ t.freeVar i = true) ->
+  ¬ t = s.up c n
+:= by
+  intro H contra
+  induction t generalizing c n s with
+  | var x =>
+    simp [freeVar] at H
+    cases s <;> try cases contra
+    grind
+  | app t1 t2 IH1 IH2 =>
+    simp [freeVar] at H
+    obtain ⟨i, H1, H2, H⟩ := H
+    cases s
+    case var | abs => cases contra
+    simp [up] at contra
+    rename_i s1 s2
+    grind
+  | abs t IH =>
+    simp [freeVar] at H
+    obtain ⟨i, H1, H2, H⟩ := H
+    cases s
+    case var | app => cases contra
+    rename_i s
+    simp [up] at contra
+    let i' := i + 1
+    replace H1: c + 1 ≤ i' := by omega
+    replace H2: i' < (c + 1) + n := by omega
+    apply IH
+    . exists i'
+    . exact contra
+
+
+theorem Tm.free_not_up0 {t s: Tm}:
+  t.freeVar 0 = true ->
+  ¬ t = s.up0
+:= by
+  intro H
+  apply Tm.free_not_up
+  simp_all
+
+
+@[simp]
+theorem Tm.up0_not_free {t: Tm}:
+  t.up0.freeVar 0 = false
+:= by
+  cases E: t.up0.freeVar 0 with
+  | false =>
+    eq_refl
+  | true =>
+    exfalso
+    apply Tm.free_not_up0
+    . exact E
+    . eq_refl
+
+
+def Tm.doEta: Tm -> Tm
+  | .var x => .var x
+  | .app t1 t2 => t1.doEta.app t2.doEta
+  | .abs t =>
+    match t.doEta with
+    | .app t1 (.var 0) =>
+      if t1.freeVar 0 then
+        .abs (t1.app (.var 0))
+      else
+        t1.down0
+    | x => .abs x
+
+
+theorem Tm.mstep_doEta {t: Tm}:
+  t.mstep t.doEta
+:= by
+  induction t with
+  | var x =>
+    simp [doEta]
+    apply RTCl.refl
+  | app t1 t2 IH1 IH2 =>
+    simp [doEta]
+    apply mstep.app
+    . exact IH1
+    . exact IH2
+  | abs t IH =>
+    generalize E: t.doEta = n
+    match E: n with
+    | .var _ | .abs _
+    | .app _ (.abs _)
+    | .app _ (.app _ _)
+    | .app _ (.var (_ + 1)) =>
+      simp_all [doEta]
+      apply IH.abs
+    | .app t1 (.var 0) =>
+      simp_all [doEta]
+      cases E: freeVar 0 t1 with
+      | true =>
+        simp_all
+        apply IH.abs
+      | false =>
+        simp
+        obtain ⟨s, E⟩ := Tm.not_free_up0 E
+        simp_all
+        apply RTCl.trans
+        . apply IH.abs
+        apply RTCl.inclusion
+        apply step.eta
+
+
+theorem Tm.BNF.doEta {t: Tm}:
+  t.BNF -> t.doEta.normal
+:= by
+  intro N
+  induction t with
+  | var x =>
+    simp [Tm.doEta] at *
+    intro ⟨_, contra⟩
+    contradiction
+  | app t1 t2 IH1 IH2 =>
+    simp [Tm.doEta]
+    cases N with | neutral N =>
+    cases N with | app N1 N2 =>
+    specialize IH1 (.neutral N1)
+    specialize IH2 N2
+    intro ⟨n, S⟩
+    have N := Tm.mstep.BNE (Tm.mstep_doEta) N1
+    clear N1 N2
+    generalize t1.doEta = t1 at *
+    generalize t2.doEta = t2 at *
+    cases S with
+    | app1 =>
+      apply IH1
+      grind
+    | app2 =>
+      apply IH2
+      grind
+    | appAbs =>
+      cases N
+  | abs t IH =>
+    cases N <;> try contradiction
+    rename_i N
+    specialize IH N
+    generalize E: t.doEta = n
+    match E: n with
+    | .var _ =>
+      simp_all [Tm.doEta]
+      intro ⟨_, S⟩
+      contradiction
+    | .abs _
+    | .app _ (.abs _)
+    | .app _ (.app _ _)
+    | .app _ (.var (_ + 1)) =>
+      simp_all [Tm.doEta]
+      intro ⟨_, S⟩
+      cases S with | abs S =>
+      apply IH
+      grind
+    | .app t1 (.var 0) =>
+      simp_all [Tm.doEta]
+      cases E: freeVar 0 t1 with
+      | true =>
+        simp
+        intro ⟨w, S⟩
+        cases S with
+        | abs S =>
+          apply IH
+          grind
+        | eta =>
+          simp_all
+      | false =>
+        simp
+        obtain ⟨s, E⟩ := Tm.not_free_up0 E
+        simp_all
+        intro ⟨_, S⟩
+        apply IH
+        constructor
+        apply step.app1
+        apply S.up
+
+
+theorem Tm.BNF.halts {t: Tm}:
+  t.BNF -> exists n: Tm, t.mstep n ∧ n.normal
+:= by
+  intro N
+  exists t.doEta
+  and_intros
+  . apply Tm.mstep_doEta
+  . apply N.doEta
+
+
+theorem Tm.N_to_BN {Γ} {t: Tm} {T}:
+  (Tm.NE Γ t T -> t.BNE) ∧ (Tm.NF Γ t T -> t.BNF)
+:= by
+  induction t generalizing Γ T with
+  | _ =>
+    grind [Tm.NE, Tm.NF, BNE, BNF]
+
+
+theorem Tm.NE.BNE {Γ t T}:
+  Tm.NE Γ t T -> t.BNE
+:= by
+  apply Tm.N_to_BN.left
+
+
+theorem Tm.NF.BNF {Γ t T}:
+  Tm.NF Γ t T -> t.BNF
+:= by
+  apply Tm.N_to_BN.right
+
+
+theorem Tm.normalizing {Γ} {t: Tm} {T}:
+  Tm.NF Γ t T -> exists n: Tm, t.mstep n ∧ n.normal
+:= by
+  intro N
+  apply Tm.BNF.halts
+  apply N.BNF
+
+
+
+/--
+The parallel reduction relation.
+-/
+inductive Tm.step2: Tm -> Tm -> Prop where
+  -- beta reduction
+  | appAbs {t1 t2 s1 s2: Tm}: t1.step2 t2 -> s1.step2 s2 -> Tm.step2 (.app t1.abs s1) (t2.subst 0 s2.up0).down0
+  -- eta
+  | eta {t1 t2: Tm}: t1.step2 t2 -> (t1.up0.app (.var 0)).abs.step2 t2
+  -- congrunence relation
+  | abs {t1 t2: Tm}: Tm.step2 t1 t2 -> Tm.step2 t1.abs t2.abs
+  | app {t1 t2 s1 s2: Tm}: Tm.step2 t1 t2 -> Tm.step2 s1 s2 -> Tm.step2 (.app t1 s1) (.app t2 s2)
+  -- refl
+  | var {x: Nat}: Tm.step2 (.var x) (.var x)
+
+
+theorem Tm.step2.refl {t: Tm}:
+  t.step2 t
+:= by
+  induction t <;> grind [Tm.step2]
+
+
+theorem Tm.step2.app1 {t1 t2 s: Tm}:
+  t1.step2 t2 ->
+  (t1.app s).step2 (t2.app s)
+:= by
+  intro S
+  apply app
+  . exact S
+  . apply refl
+
+
+theorem Tm.step2.app2 {t s1 s2: Tm}:
+  s1.step2 s2 ->
+  (t.app s1).step2 (t.app s2)
+:= by
+  intro S
+  apply app
+  . apply refl
+  . exact S
+
+
+theorem Tm.step.step2 {t1 t2: Tm}:
+  t1.step t2 -> t1.step2 t2
+:= by
+  intro S
+  induction S with
+  | appAbs =>
+    apply step2.appAbs .refl .refl
+  | abs S IH =>
+    apply step2.abs
+    apply IH
+  | app1 S IH =>
+    apply step2.app1
+    exact IH
+  | app2 S IH =>
+    apply step2.app2
+    exact IH
+  | eta =>
+    apply step2.eta
+    apply step2.refl
+
+
+theorem Tm.step2.mstep {t1 t2: Tm}:
+  t1.step2 t2 -> t1.mstep t2
+:= by
+  intro S
+  induction S with
+  | var =>
+    apply RTCl.refl
+  | appAbs S1 S2 IH1 IH2 =>
+    apply RTCl.trans
+    . apply Tm.mstep.app1
+      apply Tm.mstep.abs
+      apply IH1
+    apply RTCl.trans
+    . apply Tm.mstep.app2
+      apply IH2
+    apply RTCl.inclusion
+    apply step.appAbs
+  | eta S IH =>
+    apply RTCl.step
+    . apply step.eta
+    . exact IH
+  | abs S IH =>
+    apply mstep.abs
+    exact IH
+  | app S1 S2 IH1 IH2 =>
+    apply mstep.app
+    . apply IH1
+    . apply IH2
+
+
+theorem Tm.step2.compute {t t' t'': Tm}:
+  t.step2 t' -> t' = t'' -> t.step2 t''
+:= by
+  intro H E
+  simp_all
+
+
+theorem Tm.step2.ssubst {t1 t2: Tm} {s: Subst}:
+  t1.step2 t2 ->
+  (t1.ssubst s).step2 (t2.ssubst s)
+:= by
+  intro S
+  induction S generalizing s with
+  | var =>
+    apply step2.refl
+  | abs S IH =>
+    simp [Tm.ssubst]
+    apply step2.abs
+    apply IH
+  | app S1 S2 IH1 IH2 =>
+    simp [Tm.ssubst]
+    apply step2.app
+    . apply IH1
+    . apply IH2
+  | appAbs S1 S2 IH1 IH2 =>
+    simp [Tm.ssubst]
+    apply Tm.step2.compute
+    . apply appAbs
+      . apply IH1
+      . apply IH2
+    simp [Tm.step_ssubst]
+    apply Tm.ssubst_congr
+    intro n
+    simp [Subst.comp]
+    cases n with
+    | zero =>
+      simp [Subst.abs, Tm.ssubst, Subst.step]
+    | succ =>
+      simp [Subst.abs, Tm.ssubst, Subst.step]
+  | eta S IH =>
+    simp [Tm.ssubst]
+    apply Tm.step2.compute
+    . apply eta
+      apply IH
+    eq_refl
+
+
+theorem Tm.step2.subst1 {t1 t2 s: Tm} {i}:
+  t1.step2 t2 ->
+  (t1.subst i s).step2 (t2.subst i s)
+:= by
+  simp [Tm.subst_ssubst]
+  apply Tm.step2.ssubst
+
+
+theorem Tm.step2.up {t1 t2: Tm} {c n}:
+  t1.step2 t2 -> (t1.up c n).step2 (t2.up c n)
+:= by
+  simp [Tm.up_ssubst]
+  apply Tm.step2.ssubst
+
+
+theorem Tm.step2.down {t1 t2: Tm} {c}:
+  t1.step2 t2 -> (t1.down c).step2 (t2.down c )
+:= by
+  simp [Tm.down_ssubst]
+  apply Tm.step2.ssubst
+
+
+theorem Tm.step2.subst2 {t s1 s2: Tm} {i}:
+  s1.step2 s2 ->
+  (t.subst i s1).step2 (t.subst i s2)
+:= by
+  intro S
+  induction t generalizing i s1 s2 with
+  | var x =>
+    simp [Tm.subst]
+    split
+    . exact S
+    . apply step2.refl
+  | abs t IH =>
+    simp [Tm.subst]
+    apply step2.abs
+    apply IH
+    apply S.up
+  | app t1 t2 IH1 IH2 =>
+    simp [Tm.subst]
+    apply Tm.step2.app
+    . apply IH1
+      exact S
+    . apply IH2
+      exact S
+
+
+theorem Tm.not_free_subst_eq {t s: Tm} {i: Nat}:
+  t.freeVar i = false ->
+  t.subst i s = t
+:= by
+  induction t generalizing i s with
+  | var x =>
+    simp [freeVar, subst]
+    grind
+  | app t1 t2 IH1 IH2 =>
+    simp [freeVar, subst]
+    grind
+  | abs t IH =>
+    simp [freeVar, subst]
+    grind
+
+
+@[simp]
+theorem Tm.up0_subst_eq {t s: Tm}:
+  t.up0.subst 0 s = t.up0
+:= by
+  apply Tm.not_free_subst_eq
+  simp
+
+
+theorem Tm.subst_up0 {t s: Tm} {i}:
+  (t.up0.subst (i + 1) s.up0) = (t.subst i s).up0
+:= by
+  unfold up0
+  simp [Tm.up_ssubst, Tm.subst_ssubst]
+  apply Tm.ssubst_congr
+  intro n
+  simp [Subst.comp, Subst.term, Subst.up, ssubst]
+  split
+  . eq_refl
+  . simp [Subst.up, ssubst]
+
+
+theorem Tm.step2.subst {t1 t2 s1 s2: Tm} {i}:
+  t1.step2 t2 ->
+  s1.step2 s2 ->
+  (t1.subst i s1).step2 (t2.subst i s2)
+:= by
+  intro S1 S2
+  induction S1 generalizing i s1 s2 with
+  | var =>
+    apply step2.subst2
+    exact S2
+  | abs S IH =>
+    simp [Tm.subst]
+    apply step2.abs
+    apply IH
+    apply S2.up
+  | app _ _ IH1 IH2 =>
+    simp [Tm.subst]
+    apply step2.app
+    . apply IH1
+      exact S2
+    . apply IH2
+      exact S2
+  | appAbs _ _ IH1 IH2 =>
+    simp [Tm.subst]
+    apply step2.compute
+    . apply step2.appAbs
+      . apply IH1
+        exact S2.up
+      . apply IH2
+        exact S2
+    simp [Tm.step_ssubst]
+    simp [Tm.subst_ssubst, Tm.up_ssubst]
+    apply Tm.ssubst_congr
+    intro n
+    simp [Subst.comp]
+    induction n with
+    | zero =>
+      simp [Tm.ssubst, Subst.term, Subst.step]
+    | succ n =>
+      simp [Tm.ssubst, Subst.term, Subst.step]
+      split
+      . simp
+        rewrite [Tm.ssubst_id s2]
+        simp
+        apply Tm.ssubst_congr
+        intro n
+        simp [Subst.comp]
+        simp [Subst.id, Tm.ssubst, Subst.step, Subst.comp, Subst.up]
+      . simp [Tm.ssubst, Subst.step]
+  | eta S IH =>
+    rename_i t1 t2
+    simp [Tm.subst]
+    simp [Tm.subst_up0]
+    apply step2.eta
+    apply IH
+    exact S2
+
+
+def Tm.eval (t: Tm): Tm :=
+  match t with
+  | .var x => .var x
+  | .app (.abs t1) t2 => (t1.eval.subst 0 t2.eval.up0).down0
+  | .app t1 t2 => .app t1.eval t2.eval
+  | .abs (.app t1 (.var 0)) =>
+    if t1.freeVar 0 then .abs (t1.app (.var 0)).eval else t1.down0.eval
+  | .abs t => .abs t.eval
+termination_by t.size
+decreasing_by
+  all_goals (try grind [size])
+  simp [size]
+  omega
+
+
+@[simp]
+theorem Tm.eval_up_eta {t: Tm}:
+  (t.up0.app (Tm.var 0)).abs.eval = t.eval
+:= by
+  simp [eval]
+
+
+theorem Tm.step2_eval {t: Tm}:
+  t.step2 t.eval
+:= by
+  induction t using strong_ind with
+  | var x =>
+    simp [eval]
+    apply step2.refl
+  | abs t IH =>
+    unfold eval
+    split <;> try contradiction
+    next E =>  -- eta reduction
+      cases t <;> try cases E
+      rename_i t
+      split
+      . apply step2.abs
+        apply IH
+        simp [size]
+      . simp_all
+        obtain ⟨s, E⟩ := Tm.not_free_up0 (by assumption)
+        simp_all
+        apply step2.eta
+        apply IH
+        simp [size]
+        omega
+    next E => -- otherwise
+      specialize IH t (by grind [size])
+      simp_all
+      apply IH.abs
+  | app t1 t2 IH =>
+    have IH1 := IH t1 (by grind [size])
+    have IH2 := IH t2 (by grind [size])
+    cases t1 with
+    | var x =>
+      simp [eval]
+      apply step2.app2
+      exact IH2
+    | app s1 s2 =>
+      simp [eval]
+      apply step2.app
+      . apply IH1
+      . apply IH2
+    | abs t1 =>
+      simp [eval]
+      apply step2.appAbs
+      . apply IH
+        grind [size]
+      . apply IH
+        grind [size]
+
+
+
+theorem Tm.not_free_up_not_free {t: Tm} {c n: Nat} {x}:
+  t.freeVar x = false <-> (t.up c n).freeVar (Rename.up c n x) = false
+:= by
+  induction t generalizing c n x with
+  | var =>
+    grind [freeVar, Rename.up, Tm.up]
+  | app =>
+    grind [freeVar, Rename.up, Tm.up]
+  | abs t IH =>
+    simp [freeVar, Rename.up, Tm.up] at *
+    have E: (x < c) = (x + 1 < c + 1) := by grind
+    specialize IH (c := c + 1) (x := x + 1) (n := n)
+    grind
+
+
+theorem Tm.step_not_free {t s: Tm} {x c: Nat}:
+  t.freeVar (Rename.up c 1 x) = false ->
+  s.freeVar x = false ->
+  ((t.subst c (s.up c 1)).down c).freeVar x = false
+:= by
+  intro H1 H2
+  induction t generalizing c s x with
+  | var y =>
+    simp [subst, freeVar, Rename.up] at *
+    split
+    . simp
+      exact H2
+    . simp [freeVar, down]
+      grind
+  | app t1 t2 IH1 IH2 =>
+    simp [freeVar, subst, down] at *
+    grind
+  | abs t IH =>
+    simp [freeVar, subst, down] at *
+    rewrite [Tm.up0_switch]
+    apply IH
+    . simp [Rename.up] at *
+      grind
+    . replace H2 := (not_free_up_not_free (c := 0) (n := 1)).mp H2
+      simp [Rename.up] at H2
+      apply H2
+
+
+theorem Tm.step2.not_free {t s: Tm} {x: Nat}:
+  t.step2 s ->
+  t.freeVar x = false ->
+  s.freeVar x = false
+:= by
+  intro S H
+  induction S generalizing x with
+  | var =>
+    simp [freeVar] at *
+    trivial
+  | app S1 S2 IH1 IH2 =>
+    simp [freeVar] at *
+    grind
+  | abs S IH =>
+    rename_i t s
+    simp [freeVar] at *
+    apply IH
+    exact H
+  | appAbs S1 S2 IH1 IH2 =>
+    rename_i t1 s1 t2 s2
+    simp [freeVar] at H
+    obtain ⟨H1, H2⟩ := H
+    specialize IH1 H1
+    specialize IH2 H2
+    apply Tm.step_not_free
+    simp [Rename.up]
+    . exact IH1
+    . exact IH2
+  | eta S IH =>
+    rename_i t s
+    simp [freeVar] at H
+    apply IH
+    apply (Tm.not_free_up_not_free (c := 0) (n := 1)).mpr
+    simp [Rename.up]
+    apply H
+
+
+theorem Tm.step2.switch {t s: Tm}:
+  t.step2 s ->
+  s.step2 t.eval
+:= by
+  intro S
+  induction t using Tm.strong_ind generalizing s with
+  | var x =>
+    cases S
+    simp [eval]
+    apply step2.var
+  | app t1 t2 IH =>
+    cases S with
+    | app S1 S2 =>
+      rename_i s1 s2
+      have IH1 := IH t1 (by grind [size]) S1
+      have IH2 := IH t2 (by grind [size]) S2
+      unfold eval
+      split <;> try contradiction
+      next E => -- β-redex
+        simp_all; clear E
+        rename_i t1 t2
+        cases S1 with
+        | abs S1 =>
+          rename_i s1
+          replace IH1 := IH t1 (by grind [size]) S1
+          apply step2.appAbs
+          . exact IH1
+          . exact IH2
+        | eta S1 =>
+          rename_i t1
+          simp at IH1
+          have E: (s1.up0.app s2.up0) = (s1.up0.app (.var 0)).subst 0 s2.up0 := by
+            simp [Tm.subst]
+          replace E := congrArg Tm.down0 E
+          simp at E
+          rewrite [E]
+          apply step2.down
+          apply Tm.step2.subst
+          . apply IH
+            . grind [size]
+            . apply step2.app1
+              apply S1.up
+          . apply IH2.up
+      next => -- otherwise
+        simp_all
+        apply step2.app
+        . exact IH1
+        . exact IH2
+    | appAbs S1 S2 =>
+      rename_i t1 s1 s2
+      -- we need it for
+      have IH1 := IH t1 (by grind [size]) S1
+      have IH2 := IH t2 (by grind [size]) S2
+      simp [eval]
+      apply step2.down
+      apply step2.subst
+      . apply IH1
+      . apply IH2.up
+  | abs t IH =>
+    cases S with
+    | eta S =>
+      rename_i t
+      simp
+      apply IH
+      . simp [size]
+        omega
+      . exact S
+    | abs S =>
+      rename_i s
+      unfold eval
+      split <;> try contradiction
+      next E => -- app
+        simp_all; clear E
+        rename_i t
+        split
+        . -- not a η-redex
+          apply step2.abs
+          apply IH (t.app (.var 0))
+          . grind [size]
+          . exact S
+        . rename_i N
+          simp_all
+          cases S with
+          | app S1 S2 =>
+            rename_i s _
+            cases S2
+            replace N := S1.not_free N
+            obtain ⟨s, E⟩ := Tm.not_free_up0 N
+            simp_all; clear E
+            apply step2.eta
+            apply IH
+            . simp [size]
+              omega
+            . replace S1 := S1.down (c := 0)
+              simp [up0] at S1
+              exact S1
+          | appAbs S1 S2 =>
+            rename_i t s _
+            cases S2
+            apply IH _ (by simp [size])
+            simp [down0, Tm.down]
+            apply step2.abs
+            simp [freeVar] at N
+            have E: t.down 1 = t.down 0 := by
+              clear S1 IH
+              rewrite [<-Nat.add_zero 1] at *
+              generalize 0 = c at *
+              induction t generalizing c <;>
+              . grind [Tm.down, freeVar]
+            rewrite [E]
+            apply S1.down
+      next E => -- not a η-redex
+        simp_all; clear E
+        apply step2.abs
+        apply IH
+        . grind [size]
+        . exact S
+
+
+theorem Tm.step2.eval {t1 t2: Tm}:
+  t1.step2 t2 ->
+  t1.eval.step2 t2.eval
+:= by
+  intro S
+  replace S := S.switch
+  apply S.switch
+
+
+theorem Tm.mstep.eval {t1 t2: Tm}:
+  t1.mstep t2 -> t1.eval.mstep t2.eval
+:= by
+  intro S
+  induction S with
+  | refl =>
+    apply RTCl.refl
+  | step Hxy Hyz IH =>
+    replace Hxy := Hxy.step2
+    replace Hxy := Hxy.eval
+    replace Hxy := Hxy.mstep
+    apply RTCl.trans
+    . apply Hxy
+    . apply IH
+
+
+instance Tm.step.semi_confl: SemiConfluent Tm.step where
+  semi_confl := by
+    intro m1 m2 m3 S MS
+    exists m3.eval
+    and_intros
+    . replace S := S.step2
+      replace S := S.switch
+      replace S := S.mstep
+      apply RTCl.trans
+      . apply S
+      . apply mstep.eval
+        exact MS
+    . apply step2.mstep
+      apply step2_eval
+
+
+theorem Tm.eq.normal_same {t1 t2: Tm}:
+  t1.eq t2 -> t1.normal -> t2.normal -> t1 = t2
+:= by
+  intro E N1 N2
+  obtain ⟨s, H1s, H2s⟩ := ChurchRosser.church_rosser E
+  replace N1 := N1.MNormal H1s
+  replace N2 := N2.MNormal H2s
+  simp_all
+
+
+theorem Tm.eq.doEta {t1 t2: Tm}:
+  t1.eq t2 -> t1.doEta.eq t2.doEta
+:= by
+  intro E
+  apply ECl.trans
+  . apply ECl.symm
+    apply RTCl.sub_ecl
+    apply Tm.mstep_doEta
+  apply ECl.trans
+  . exact E
+  apply RTCl.sub_ecl
+  . apply Tm.mstep_doEta
+
+
+theorem Tm.eq.doEta_inv {t1 t2: Tm}:
+  t1.doEta.eq t2.doEta -> t1.eq t2
+:= by
+  intro E
+  apply ECl.trans
+  . apply RTCl.sub_ecl
+    apply Tm.mstep_doEta
+  apply ECl.trans
+  . exact E
+  apply ECl.symm
+  . apply RTCl.sub_ecl
+    apply Tm.mstep_doEta
+
+
+theorem Tm.eq.doEta_same {t1 t2: Tm}:
+  t1.eq t2 ->
+  t1.BNF -> t2.BNF ->
+  t1.doEta = t2.doEta
+:= by
+  intro E N1 N2
+  replace E := E.doEta
+  apply E.normal_same
+  . apply N1.doEta
+  . apply N2.doEta
+
+
+theorem Tm.abs_up_app_step {t: Tm}:
+  (t.abs.up0.app (.var 0)).step t
+:= by
+  simp [up0, up]
+  apply Tm.step.compute Tm.step.appAbs_ssubst
+  simp [Tm.up_ssubst]
+  conv =>
+    rhs
+    rewrite [Tm.ssubst_id t]
+  congr
+  funext n
+  cases n with
+  | zero =>
+    simp [Subst.comp, Subst.step, ssubst, Subst.up, Subst.id]
+  | succ =>
+    simp [Subst.comp, Subst.step, ssubst, Subst.up, Subst.id]
+
+
+theorem Tm.eq.abs_inv {t s: Tm}:
+  t.abs.eq s.abs -> t.eq s
+:= by
+  intro E
+  apply ECl.rstep
+  . apply Tm.abs_up_app_step
+  apply ECl.trans
+  . apply Tm.eq.app1
+    apply E.up
+  apply ECl.inclusion
+  apply Tm.abs_up_app_step
+
+
+theorem Tm.NE.type_unique {Γ: Context} {t: Tm} {T1 T2}:
+  Tm.NE Γ t T1 -> Tm.NE Γ t T2 -> T1 = T2
+:= by
+  intro N1 N2
+  induction t generalizing Γ T1 T2 with
+  | var x =>
+    cases N1
+    cases N2
+    simp_all
+  | app t1 t2 IH1 IH2 =>
+    cases N1 with | app N11 N12 =>
+    cases N2 with | app N21 N22 =>
+    specialize IH1 N11 N21
+    simp_all
+  | abs =>
+    cases N1
+
+
+theorem Tm.BNE.type_unique {Γ: Context} {t: Tm} {T1 T2}:
+  t.BNE ->
+  Γ.Typing t T1 -> Γ.Typing t T2 -> T1 = T2
+:= by
+  intro N HT1 HT2
+  induction t generalizing Γ T1 T2 with
+  | var x =>
+    cases HT1
+    cases HT2
+    simp_all
+  | app t1 t2 IH1 IH2 =>
+    cases N with | app N _ =>
+    cases HT1 with | app HT1 _ =>
+    cases HT2 with | app HT2 _ =>
+    specialize IH1 N HT1 HT2
+    simp_all
+  | abs =>
+    cases N
+
+
+theorem Tm.BNE.eq_type_unique {Γ: Context} {t s: Tm} {T1 T2}:
+  t.eq s -> t.BNE -> s.BNE ->
+  Γ.Typing t T1 -> Γ.Typing s T2 -> T1 = T2
+:= by
+  intro E N1 N2 HT1 HT2
+  replace HT1: Γ.Typing t.doEta T1 := by
+    apply Tm.mstep.typing
+    apply Tm.mstep_doEta
+    exact HT1
+  replace HT2: Γ.Typing s.doEta T2 := by
+    apply Tm.mstep.typing
+    apply Tm.mstep_doEta
+    exact HT2
+  replace E := E.doEta_same N1.BNF N2.BNF
+  rewrite [E] at HT1
+  have N: s.doEta.BNE := by
+    apply Tm.mstep.BNE
+    apply Tm.mstep_doEta
+    exact N2
+  apply N.type_unique
+  . exact HT1
+  . exact HT2
+
+
+theorem Tm.N_uniqueness {Γ} {t s: Tm} {T}:
+  t.eq s ->
+  (Tm.NF Γ t T -> Tm.NF Γ s T -> t = s) ∧ (Tm.NE Γ t T -> Tm.NE Γ s T -> t = s)
+:= by
+  intro E
+  induction t generalizing s Γ T with
+  | var x =>
+    have H: (Tm.NE Γ (var x) T -> Tm.NE Γ s T -> (var x) = s) := by
+      intro N1 N2
+      cases s with
+      | abs =>
+        cases N2
+      | app s1 s2 =>
+        replace E := E.doEta_same N1.BNE.BNF N2.BNE.BNF
+        simp [doEta] at E
+      | var y =>
+        replace E := E.doEta_same N1.BNE.BNF N2.BNE.BNF
+        simp_all [doEta]
+    and_intros
+    . intro N1 N2
+      cases N1 with | atom N1 =>
+      cases N2 with | atom N2 =>
+      solve_by_elim
+    . apply H
+  | app t1 t2 IH1 IH2 =>
+    have H: (Tm.NE Γ (t1.app t2) T -> Tm.NE Γ s T -> (t1.app t2) = s) := by
+      intro N1 N2
+      cases s with
+      | abs =>
+        cases N2
+      | var x =>
+        replace E := E.doEta_same N1.BNE.BNF N2.BNE.BNF
+        simp [doEta] at E
+      | app s1 s2 =>
+        replace E := E.doEta_same N1.BNE.BNF N2.BNE.BNF
+        simp [doEta] at E
+        obtain ⟨E1, E2⟩ := E
+        replace E1: t1.eq s1 := by
+          apply Tm.eq.doEta_inv
+          rewrite [E1]
+          apply ECl.refl
+        replace E2: t2.eq s2 := by
+          apply Tm.eq.doEta_inv
+          rewrite [E2]
+          apply ECl.refl
+        -- Normality
+        cases N1 with | app N11 N12 =>
+        cases N2 with | app N21 N22 =>
+        -- which forces the type
+        have E := Tm.BNE.eq_type_unique E1 N11.BNE N21.BNE N11.typing N21.typing
+        cases E
+        replace IH1 := (IH1 E1).right N11 N21
+        replace IH2 := (IH2 E2).left N12 N22
+        simp_all
+    and_intros
+    . intro N1 N2
+      cases N1 with | atom N1 =>
+      cases N2 with | atom N2 =>
+      solve_by_elim
+    . apply H
+  | abs t IH =>
+    and_intros
+    . intro N1 N2
+      cases N1 <;> try contradiction
+      rename_i T1 T2 N1
+      cases N2 with | abs N2 =>
+      rename_i s
+      replace E := E.abs_inv
+      replace IH := (IH E).left N1 N2
+      simp_all
+    . intro N
+      cases N
