NBE/SingleSortImp/BetaEtaNormalizing.lean
@@ -1,0 +1,120 @@
+import NBE.SingleSortImp.BetaEta
+import NBE.SingleSortImp.Presheaf
+
+namespace SingleSortImp
+namespace BetaEtaNormalizing
+
+
+def NE: Presheaf where
+  Pred Γ t T := exists t', t.eq t' ∧ Tm.NE Γ t' T
+  weaken {Γ' Γ t T} := by
+    rintro ⟨t', E, N⟩
+    exists t'.up 0 Γ'.length
+    and_intros
+    . apply E.up
+    . apply N.weaken_app
+
+
+def NF: Presheaf where
+  Pred Γ t T := exists t', t.eq t' ∧ Tm.NF Γ t' T
+  weaken {Γ' Γ t T} := by
+    rintro ⟨t', E, N⟩
+    exists t'.up 0 Γ'.length
+    and_intros
+    . apply E.up
+    . apply N.weaken_app
+
+
+
+instance: NF.HasNeutral where
+  NE := NE
+  atom {Γ t} := by
+    intro H
+    simp [NE, NF] at *
+    rcases H with ⟨t', E, N⟩
+    exists t'
+    and_intros
+    . exact E
+    . apply Tm.NF.atom
+      exact N
+  var {Γ T} := by
+    simp [NE]
+    exists (.var 0)
+    and_intros
+    . apply ECl.refl
+    . apply Tm.NE.var
+      simp
+  imp {Γ Γ' t s A B} := by
+    rintro ⟨t', Et', Nt'⟩
+    rintro ⟨s', Es', Ns'⟩
+    exists (t'.up 0 Γ'.length).app s'
+    and_intros
+    . apply Tm.eq.app
+      . apply Et'.up
+      . exact Es'
+    . apply Tm.NE.app
+      . apply Nt'.weaken_app
+      . exact Ns'
+  app_inv {Γ t A B} := by
+    rintro ⟨t', E, N⟩
+    exists t'.abs
+    and_intros
+    . apply ECl.rstep
+      . apply Tm.step.eta
+      . apply Tm.eq.abs
+        exact E
+    . apply Tm.NF.abs
+      exact N
+
+
+theorem step_forces' {Γ: Context} {t t': Tm} {T}:
+  t.step t' ->
+  NF.forces Γ t' T ->
+  NF.forces Γ t T
+:= by
+  intro S F
+  induction T generalizing Γ t t' with
+  | Atom =>
+    simp [Presheaf.forces, forcePred] at *
+    obtain ⟨t'', S', N⟩ := F
+    exists t''
+    and_intros
+    . apply ECl.step
+      . exact S
+      . exact S'
+    . exact N
+  | imp T1 T2 IH1 IH2 =>
+    simp [Presheaf.forces, forcePred] at *
+    intro s Γ' F'
+    apply IH2
+    . apply Tm.step.app1
+      apply Tm.step.up
+      exact S
+    . apply F
+      exact F'
+
+
+instance: NF.MSubst where
+  msubst {Γ t T1 T2 Δ Δ' s env} HT I N F := by
+    apply step_forces' _ F
+    simp [Tm.up, Tm.msubst]
+    apply Tm.step.compute
+    . apply Tm.step.appAbs
+    apply Tm.msubst_le_step
+    generalize Δ'.length = n
+    replace HT := HT.bound
+    simp_all [I.length]
+
+
+/--
+This is the result of the real completeness
+-/
+theorem Tm.NF_halts {Γ: Context} {t T}:
+  Γ.Typing t T -> exists t', t.eq t' ∧ Tm.NF Γ t' T
+:= by
+  intro HT
+  let entailment := NF.soundness HT
+  specialize entailment Γ (Env.vars Γ.length) Instantiate.self
+  simp at entailment
+  apply NF.completeness
+  exact entailment
